theories/Eq/Trans.v
@@ -34,8 +34,7 @@ closed under [equ] rather than [eq].
 
 From Coq Require Import Fin.
 
-From Coinduction Require Import
-     coinduction rel tactics.
+From Coinduction Require Import all.
 
 From ITree Require Import
      Core.Subevent
@@ -73,7 +72,6 @@ Set Primitive Projections.
 Section Trans.
 
   Context {E B : Type -> Type} {R : Type}.
-  Context {HasStuck: B0 -< B}.
 
   Notation S' := (ctree' E B R).
   Notation S  := (ctree  E B R).
@@ -89,14 +87,14 @@ be of type [R]. However typing it statically makes lemmas about
 least annoying solution.
 |*)
   Variant label : Type :=
-    | tau
+    | τ
     | obs {X : Type} (e : E X) (v : X)
     | val {X : Type} (v : X).
 
   Variant is_val : label -> Prop :=
     | Is_val : forall X (x : X), is_val (val x).
 
-  Lemma is_val_tau : ~ is_val tau.
+  Lemma is_val_τ : ~ is_val τ.
   Proof.
     intro H. inversion H.
   Qed.
@@ -117,20 +115,24 @@ node, labelling the transition by the returned value.
 |*)
   Inductive trans_ : label -> hrel S' S' :=
 
-  | Stepbr {X} (c : B X) x k l t :
+  | Transbr {X} (c : B X) x k l t :
     trans_ l (observe (k x)) t ->
-    trans_ l (BrF false c k) t
+    trans_ l (BrF c k) t
 
-  | Steptau {X} (c : B X) x k t :
-    k x ≅ t ->
-    trans_ tau (BrSF c k) (observe t)
+  | Transguard t t' l :
+    trans_ l (observe t) t' ->
+    trans_ l (GuardF t) t'
 
-  | Stepobs {X} (e : E X) k x t :
+  | Transtau t u :
+    u ≅ t ->
+    trans_ τ (StepF t) (observe u)
+
+  | Transobs {X} (e : E X) k x t :
     k x ≅ t ->
     trans_ (obs e x) (VisF e k) (observe t)
 
-  | Stepval r k :
-    trans_ (val r) (RetF r) (brDF branch0 k).
+  | Transval r :
+    trans_ (val r) (RetF r) StuckF.
   Hint Constructors trans_ : core.
 
   Definition transR l : hrel S S :=
@@ -153,19 +155,31 @@ node, labelling the transition by the returned value.
     + inv equ.
       * rewrite H2; eauto.
       * FtoObs.
-	apply (Steptau c x).
-	rewrite H.
-	rewrite (ctree_eta t), <- H2.
-	step; constructor; intros; symmetry; auto.
+        constructor.
+        rewrite <- H.
+        apply observing_sub_equ; eauto.
       * FtoObs.
-	apply (Steptau c x).
-	rewrite H.
-	rewrite (ctree_eta t), <- H2.
-	step; constructor; intros; symmetry; auto.
-    + FtoObs.
+        constructor.
+        rewrite <- H, REL.
+        apply observing_sub_equ; eauto.
+      * FtoObs.
+        constructor.
+        rewrite <- H, REL.
+        apply observing_sub_equ; eauto.
+      * FtoObs.
+        constructor.
+        rewrite <- H.
+        step; rewrite <- H2; constructor; intros.
+        auto.
+      * FtoObs.
+        constructor.
+        rewrite <- H.
+        step; rewrite <- H2; constructor; intros.
+        auto.
+   + FtoObs.
       econstructor.
       rewrite H; symmetry; step; auto.
-    + inv equ. dependent destruction H3. econstructor.
+    + inv equ. eauto.
   Qed.
 
   #[local] Instance trans_equ_aux2 l :
@@ -177,12 +191,14 @@ node, labelling the transition by the returned value.
     revert t' eqt.
     dependent induction TR; intros; auto.
     + step in eqt; dependent induction eqt.
-      apply (Stepbr c x).
+      econstructor.
       apply IHTR.
       rewrite REL; reflexivity.
     + step in eqt; dependent induction eqt.
       econstructor.
-      rewrite <- REL; eauto.
+      apply IHTR. rewrite REL; reflexivity.
+    + step in eqt; dependent induction eqt.
+      econstructor. rewrite H,REL; auto.
     + step in eqt; dependent induction eqt.
       econstructor.
       rewrite <- REL; eauto.
@@ -198,7 +214,7 @@ node, labelling the transition by the returned value.
     - symmetry in equ; symmetry in eqt; eapply trans_equ_aux2; eauto.
   Qed.
 
-  (*|
+(*|
 [equ] is congruent for [trans], we can hence build a [srel] and build our
 relations in this model to still exploit the automation from the [RelationAlgebra]
 library.
@@ -224,27 +240,27 @@ library.
     reflexivity.
   Qed.
 
-  (*|
-Extension of [trans] with its reflexive closure, labelled by [tau].
+(*|
+Extension of [trans] with its reflexive closure, labelled by [τ].
 |*)
   Definition etrans (l : label) : srel SS SS :=
     match l with
-    | tau => (cup (trans l) 1)
+    | τ => (cup (trans l) 1)
     | _ => trans l
     end.
 
-  (*|
+(*|
 The transition for the weak bisimulation: a sequence of
 internal steps, a labelled step, and a new sequence of internal ones
 |*)
   Definition wtrans l : srel SS SS :=
-    (trans tau)^* ⋅ etrans l ⋅ (trans tau)^*.
+    (trans τ)^* ⋅ etrans l ⋅ (trans τ)^*.
 
   Definition pwtrans l : srel SS SS :=
-    (trans tau)^* ⋅ trans l ⋅ (trans tau)^*.
+    (trans τ)^* ⋅ trans l ⋅ (trans τ)^*.
 
-  Definition tautrans : srel SS SS :=
-    (trans tau)^+.
+  Definition τtrans : srel SS SS :=
+    (trans τ)^+.
 
   (*|
 ----------------------------------------------
@@ -255,25 +271,25 @@ Inclusion relation between the three relations:
 [trans l ≤ etrans l ≤ wtrans l]
 
 [etrans] is reflexive, and hence so is [wtrans]
-[etrans tau p p]
+[etrans τ p p]
 
-[wtrans] can be built by consing or snocing [trans tau]
-[trans tau p p' -> wtrans l p' p'' -> wtrans l p p'']
-[wtrans l p p' -> trans tau p' p'' -> wtrans l p p'']
+[wtrans] can be built by consing or snocing [trans τ]
+[trans τ p p' -> wtrans l p' p'' -> wtrans l p p'']
+[wtrans l p p' -> trans τ p' p'' -> wtrans l p p'']
 
 Introduction rules for [trans]
 [trans (val v)   (ret v)       stuck]
 [trans (obs e v) (Vis e k)     (k v)]
-[trans tau       (BrS n k) (k x)]
-[trans tau       (Step t) t]
+[trans τ       (BrS n k) (k x)]
+[trans τ       (Step t) t]
 [trans l (k x) u -> trans l (BrI n k) u]
 [trans l t u     -> trans l (Guard t) u]
 
 Elimination rules for [trans]
 [trans l (Ret x)       u -> l = val x /\ t ≅ stuck]
 [trans l (Vis e k)     u -> exists v, l = obs e v /\ t ≅ k v]
-[trans l (BrS n k) u -> exists x, t' ≅ k x /\ l = tau]
-[trans l (Step t)      u -> t ≅ u /\ l = tau]
+[trans l (BrS n k) u -> exists x, t' ≅ k x /\ l = τ]
+[trans l (Step t)      u -> t ≅ u /\ l = τ]
 [trans l (BrI n k) u -> exists x, trans l (k x) u]
 [trans l (Guard t)      u -> trans l t u]
 
@@ -288,9 +304,9 @@ Elimination rules for [trans]
   Qed.
   Lemma trans_wtrans l: trans l ≦ wtrans l.
   Proof. rewrite trans_etrans. apply etrans_wtrans. Qed.
-  Lemma tautrans_wtrans : tautrans ≦ wtrans tau.
+  Lemma τtrans_wtrans : τtrans ≦ wtrans τ.
   Proof.
-    unfold tautrans, wtrans, etrans; ka.
+    unfold τtrans, wtrans, etrans; ka.
   Qed.
   Lemma pwtrans_wtrans l : pwtrans l ≦ wtrans l.
   Proof.
@@ -303,57 +319,57 @@ Elimination rules for [trans]
   Proof. apply trans_wtrans. Qed.
   Lemma etrans_wtrans_ l: forall p p', etrans l p p' -> wtrans l p p'.
   Proof. apply etrans_wtrans. Qed.
-  Lemma tautrans_wtrans_ : forall p p', tautrans p p' -> wtrans tau p p'.
-  Proof. apply tautrans_wtrans. Qed.
+  Lemma τtrans_wtrans_ : forall p p', τtrans p p' -> wtrans τ p p'.
+  Proof. apply τtrans_wtrans. Qed.
   Lemma pwtrans_wtrans_ l : forall p p', pwtrans l p p' -> wtrans l p p'.
   Proof. apply pwtrans_wtrans. Qed.
 
-  Lemma enil p: etrans tau p p.
+  Lemma enil p: etrans τ p p.
   Proof. cbn. now right. Qed.
-  Lemma wnil p: wtrans tau p p.
+  Lemma wnil p: wtrans τ p p.
   Proof. apply etrans_wtrans, enil. Qed.
 
-  Lemma wcons l: forall p p' p'', trans tau p p' -> wtrans l p' p'' -> wtrans l p p''.
+  Lemma wcons l: forall p p' p'', trans τ p p' -> wtrans l p' p'' -> wtrans l p p''.
   Proof.
-    assert ((trans tau: srel SS SS) ⋅ wtrans l ≦ wtrans l) as H
+    assert ((trans τ: srel SS SS) ⋅ wtrans l ≦ wtrans l) as H
         by (unfold wtrans; ka).
     intros. apply H. eexists; eassumption.
   Qed.
-  Lemma wsnoc l: forall p p' p'', wtrans l p p' -> trans tau p' p'' -> wtrans l p p''.
+  Lemma wsnoc l: forall p p' p'', wtrans l p p' -> trans τ p' p'' -> wtrans l p p''.
   Proof.
-    assert (wtrans l ⋅ trans tau ≦ wtrans l) as H
+    assert (wtrans l ⋅ trans τ ≦ wtrans l) as H
         by (unfold wtrans; ka).
     intros. apply H. eexists; eassumption.
   Qed.
 
-  Lemma wconss l: forall p p' p'', wtrans tau p p' -> wtrans l p' p'' -> wtrans l p p''.
+  Lemma wconss l: forall p p' p'', wtrans τ p p' -> wtrans l p' p'' -> wtrans l p p''.
   Proof.
-    assert (wtrans tau ⋅ wtrans l ≦ wtrans l) as H by (unfold wtrans, etrans; ka).
+    assert (wtrans τ ⋅ wtrans l ≦ wtrans l) as H by (unfold wtrans, etrans; ka).
     intros. apply H. eexists; eassumption.
   Qed.
-  Lemma wsnocs l: forall p p' p'', wtrans l p p' -> wtrans tau p' p'' -> wtrans l p p''.
+  Lemma wsnocs l: forall p p' p'', wtrans l p p' -> wtrans τ p' p'' -> wtrans l p p''.
   Proof.
-    assert (wtrans l ⋅ wtrans tau ≦ wtrans l) as H by (unfold wtrans, etrans; ka).
+    assert (wtrans l ⋅ wtrans τ ≦ wtrans l) as H by (unfold wtrans, etrans; ka).
     intros. apply H. eexists; eassumption.
   Qed.
 
-  Lemma wtrans_tau: wtrans tau ≡ (trans tau)^*.
+  Lemma wtrans_τ: wtrans τ ≡ (trans τ)^*.
   Proof.
     unfold wtrans, etrans. ka.
   Qed.
 
-  Lemma pwtrans_tau: pwtrans tau ≡ (trans tau)^+.
+  Lemma pwtrans_τ: pwtrans τ ≡ (trans τ)^+.
   Proof.
     unfold pwtrans, etrans. ka.
   Qed.
 
-  #[global] Instance PreOrder_wtrans_tau: PreOrder (wtrans tau).
+  #[global] Instance PreOrder_wtrans_τ: PreOrder (wtrans τ).
   Proof.
     split.
-    intro. apply wtrans_tau.
-    now (apply (str_refl (trans tau)); cbn).
-    intros ?????. apply wtrans_tau. apply (str_trans (trans tau)).
-    eexists; apply wtrans_tau; eassumption.
+    intro. apply wtrans_τ.
+    now (apply (str_refl (trans τ)); cbn).
+    intros ?????. apply wtrans_τ. apply (str_trans (trans τ)).
+    eexists; apply wtrans_τ; eassumption.
   Qed.
 
 
@@ -365,10 +381,10 @@ Class Respects_val {E F} (L : rel (@label E) (@label F)) :=
       L l l' ->
       is_val l <-> is_val l' }.
 
-Class Respects_tau {E F} (L : rel (@label E) (@label F)) :=
-  { respects_tau: forall l l',
+Class Respects_τ {E F} (L : rel (@label E) (@label F)) :=
+  { respects_τ: forall l l',
       L l l' ->
-      l = tau <-> l' = tau }.
+      l = τ <-> l' = τ }.
 
 Definition eq_obs {E} (L : relation (@label E)) : Prop :=
   forall X X' e e' (x : X) (x' : X'),
@@ -379,7 +395,7 @@ Definition eq_obs {E} (L : relation (@label E)) : Prop :=
 split; intros; subst; reflexivity.
 Defined.
 
-#[global] Instance Respects_tau_eq A: @Respects_tau A A eq.
+#[global] Instance Respects_τ_eq A: @Respects_τ A A eq.
 split; intros; subst; reflexivity.
 Defined.
 
@@ -393,15 +409,13 @@ in the section above so that [eauto with trans] works smoothly.
 Section backward.
 
   Context {E B : Type -> Type} {X : Type}.
-  Context `{B0 -< B}.
-  Context `{B1 -< B}.
 
-  (*|
+(*|
 Structural rules
 |*)
 
   Lemma trans_ret : forall (x : X),
-      trans (E := E) (B := B) (val x) (Ret x) stuckD.
+      trans (E := E) (B := B) (val x) (Ret x) Stuck.
   Proof.
     intros; constructor.
   Qed.
@@ -412,40 +426,41 @@ Structural rules
     intros; constructor; auto.
   Qed.
 
-  Lemma trans_brD : forall {Y} l (t t' : ctree E B X) (c : B Y) k x,
+  Lemma trans_br : forall {Y} l (t t' : ctree E B X) (c : B Y) k x,
       trans l t t' ->
       k x ≅ t ->
-      trans l (BrD c k) t'.
+      trans l (Br c k) t'.
   Proof.
     intros * TR Eq.
-    apply Stepbr with x.
+    apply Transbr with x.
     rewrite Eq; auto.
   Qed.
 
   Lemma trans_brS : forall {Y} (c : B Y) (k : _ -> ctree E B X) x,
-      trans tau (BrS c k) (k x).
+      trans τ (BrS c k) (k x).
   Proof.
     intros.
-    apply Steptau with x; reflexivity.
+    apply Transbr with x, Transtau.
+    reflexivity.
   Qed.
 
-  (*|
+(*|
 Ad-hoc rules for pre-defined finite branching
 |*)
 
-  Variable (l : @label E) (t t' u u' v v' w w' : ctree E B X).
+  Variable (l : @label E) (t t' : ctree E B X).
 
   Lemma trans_step :
-    trans tau (Step t) t.
+    trans τ (Step t) t.
   Proof.
-    intros; apply (@trans_brS unit _ (fun _ => t) tt).
+    now econstructor.
   Qed.
 
   Lemma trans_guard :
     trans l t t' ->
     trans l (Guard t) t'.
   Proof.
-    intros * TR; eapply trans_brD; eauto; exact F1.
+    now econstructor.
   Qed.
 
 End backward.
@@ -453,172 +468,162 @@ End backward.
 Section BackwardBounded.
 
   Context {E B : Type -> Type} {X : Type}.
-  Context `{B0 -< B}.
   Context `{B2 -< B}.
   Context `{B3 -< B}.
   Context `{B4 -< B}.
   Variable (l : @label E) (t t' u u' v v' w w' : ctree E B X).
 
   Lemma trans_brS21 :
-    trans tau (brS2 t u) t.
+    trans τ (brS2 t u) t.
   Proof.
     intros.
     unfold brS2.
-    match goal with
-      |- _ (trans tau) (BrS _ ?k) ?t => exact (trans_brS _ k true)
-    end.
+    apply Transbr with true.
+    now constructor.
   Qed.
 
   Lemma trans_brS22 :
-    trans tau (brS2 t u) u.
+    trans τ (brS2 t u) u.
   Proof.
     intros.
     unfold brS2.
-    match goal with
-      |- _ (trans tau) (BrS _ ?k) ?t => exact (trans_brS _ k false)
-    end.
+    apply Transbr with false.
+    now constructor.
   Qed.
 
-  Lemma trans_brD21 :
+  Lemma trans_br21 :
     trans l t t' ->
-    trans l (brD2 t u) t'.
+    trans l (br2 t u) t'.
   Proof.
     intros * TR.
-    eapply trans_brD with (x := true); eauto.
+    eapply trans_br with (x := true); eauto.
   Qed.
 
-  Lemma trans_brD22 :
+  Lemma trans_br22 :
     trans l u u' ->
-    trans l (brD2 t u) u'.
+    trans l (br2 t u) u'.
   Proof.
     intros * TR.
-    eapply trans_brD with (x := false); eauto.
+    eapply trans_br with (x := false); eauto.
   Qed.
 
   Lemma trans_brS31 :
-    trans tau (brS3 t u v) t.
+    trans τ (brS3 t u v) t.
   Proof.
     intros.
     unfold brS3.
-    match goal with
-      |- _ (trans tau) (BrS _ ?k) ?t => exact (trans_brS _ k t31)
-    end.
+    apply Transbr with t31.
+    now constructor.
   Qed.
 
   Lemma trans_brS32 :
-    trans tau (brS3 t u v) u.
+    trans τ (brS3 t u v) u.
   Proof.
     intros.
     unfold brS3.
-    match goal with
-      |- _ (trans tau) (BrS _ ?k) ?t => exact (trans_brS _ k t32)
-    end.
+    apply Transbr with t32.
+    now constructor.
   Qed.
 
   Lemma trans_brS33 :
-    trans tau (brS3 t u v) v.
+    trans τ (brS3 t u v) v.
   Proof.
     intros.
     unfold brS3.
-    match goal with
-      |- _ (trans tau) (BrS _ ?k) ?t => exact (trans_brS _ k t33)
-    end.
+    apply Transbr with t33.
+    now constructor.
   Qed.
 
-  Lemma trans_brD31 :
+  Lemma trans_br31 :
     trans l t t' ->
-    trans l (brD3 t u v) t'.
+    trans l (br3 t u v) t'.
   Proof.
     intros * TR.
-    eapply trans_brD with (x := t31); eauto.
+    eapply trans_br with (x := t31); eauto.
   Qed.
 
-  Lemma trans_brD32 :
+  Lemma trans_br32 :
     trans l u u' ->
-    trans l (brD3 t u v) u'.
+    trans l (br3 t u v) u'.
   Proof.
     intros * TR.
-    eapply trans_brD with (x := t32); eauto.
+    eapply trans_br with (x := t32); eauto.
   Qed.
 
-  Lemma trans_brD33 :
+  Lemma trans_br33 :
     trans l v v' ->
-    trans l (brD3 t u v) v'.
+    trans l (br3 t u v) v'.
   Proof.
     intros * TR.
-    eapply trans_brD with (x := t33); eauto.
+    eapply trans_br with (x := t33); eauto.
   Qed.
 
   Lemma trans_brS41 :
-    trans tau (brS4 t u v w) t.
+    trans τ (brS4 t u v w) t.
   Proof.
     intros.
     unfold brS4.
-    match goal with
-      |- _ (trans tau) (BrS _ ?k) ?t => exact (trans_brS _ k t41)
-    end.
+    apply Transbr with t41.
+    now constructor.
   Qed.
 
   Lemma trans_brS42 :
-    trans tau (brS4 t u v w) u.
+    trans τ (brS4 t u v w) u.
   Proof.
     intros.
     unfold brS4.
-    match goal with
-      |- _ (trans tau) (BrS _ ?k) ?t => exact (trans_brS _ k t42)
-    end.
+    apply Transbr with t42.
+    now constructor.
   Qed.
 
   Lemma trans_brS43 :
-    trans tau (brS4 t u v w) v.
+    trans τ (brS4 t u v w) v.
   Proof.
     intros.
     unfold brS4.
-    match goal with
-      |- _ (trans tau) (BrS _ ?k) ?t => exact (trans_brS _ k t43)
-    end.
+    apply Transbr with t43.
+    now constructor.
   Qed.
 
   Lemma trans_brS44 :
-    trans tau (brS4 t u v w) w.
+    trans τ (brS4 t u v w) w.
   Proof.
     intros.
     unfold brS4.
-    match goal with
-      |- _ (trans tau) (BrS _ ?k) ?t => exact (trans_brS _ k t44)
-    end.
+    apply Transbr with t44.
+    now constructor.
   Qed.
 
-  Lemma trans_brD41 :
+  Lemma trans_br41 :
     trans l t t' ->
-    trans l (brD4 t u v w) t'.
+    trans l (br4 t u v w) t'.
   Proof.
     intros * TR.
-    eapply trans_brD with (x := t41); eauto.
+    eapply trans_br with (x := t41); eauto.
   Qed.
 
-  Lemma trans_brD42 :
+  Lemma trans_br42 :
     trans l u u' ->
-    trans l (brD4 t u v w) u'.
+    trans l (br4 t u v w) u'.
   Proof.
     intros * TR.
-    eapply trans_brD with (x := t42); eauto.
+    eapply trans_br with (x := t42); eauto.
   Qed.
 
-  Lemma trans_brD43 :
+  Lemma trans_br43 :
     trans l v v' ->
-    trans l (brD4 t u v w) v'.
+    trans l (br4 t u v w) v'.
   Proof.
     intros * TR.
-    eapply trans_brD with (x := t43); eauto.
+    eapply trans_br with (x := t43); eauto.
   Qed.
 
-  Lemma trans_brD44 :
+  Lemma trans_br44 :
     trans l w w' ->
-    trans l (brD4 t u v w) w'.
+    trans l (br4 t u v w) w'.
   Proof.
     intros * TR.
-    eapply trans_brD with (x := t44); eauto.
+    eapply trans_br with (x := t44); eauto.
   Qed.
 
 End BackwardBounded.
@@ -630,43 +635,42 @@ Forward reasoning for [trans]
 
 Section forward.
 
-  Context {E B : Type -> Type} `{HasStuck : B0 -< B} {X : Type}.
+  Context {E B : Type -> Type} {X : Type}.
 
-  (*|
+(*|
 Inverting equalities between labels
 |*)
 
   Lemma val_eq_invT : forall X Y x y, @val E X x = @val E Y y -> X = Y.
-    clear B HasStuck. intros * EQ.
+    clear B. intros * EQ.
     now dependent induction EQ.
   Qed.
 
   Lemma val_eq_inv : forall X x y, @val E X x = val y -> x = y.
-    clear B HasStuck. intros * EQ.
+    clear B. intros * EQ.
     now dependent induction EQ.
   Qed.
 
   Lemma obs_eq_invT : forall X Y e1 e2 v1 v2, @obs E X e1 v1 = @obs E Y e2 v2 -> X = Y.
-    clear B HasStuck. intros * EQ.
+    clear B. intros * EQ.
     now dependent induction EQ.
   Qed.
 
   Lemma obs_eq_inv : forall X e1 e2 v1 v2, @obs E X e1 v1 = @obs E X e2 v2 -> e1 = e2 /\ v1 = v2.
-    clear B HasStuck. intros * EQ.
+    clear B. intros * EQ.
     now dependent induction EQ.
   Qed.
 
-  (*|
+(*|
 Structural rules
 |*)
 
   Lemma trans_ret_inv : forall x l (t : ctree E B X),
       trans l (Ret x) t ->
-      t ≅ stuckD /\ l = val x.
+      t ≅ Stuck /\ l = val x.
   Proof.
     intros * TR; inv TR; intuition.
     rewrite ctree_eta, <- H2; auto.
-    step; constructor; intros abs; inv abs.
   Qed.
 
   Lemma trans_vis_inv : forall {Y} (e : E Y) k l (u : ctree E B X),
@@ -679,8 +683,8 @@ Structural rules
     rewrite ctree_eta, <- H4, <- ctree_eta; symmetry; auto.
   Qed.
 
-  Lemma trans_brD_inv : forall {Y} l (c : B Y) k (u : ctree E B X),
-      trans l (BrD c k) u ->
+  Lemma trans_br_inv : forall {Y} l (c : B Y) k (u : ctree E B X),
+      trans l (Br c k) u ->
       exists n, trans l (k n) u.
   Proof.
     intros * TR.
@@ -695,64 +699,75 @@ Structural rules
     induction TR; intros; inv Heqox; eauto.
   Qed.
 
-  (*|
+  Lemma trans_guard_inv : forall l (t : ctree E B X) u,
+      trans l (Guard t) u ->
+      trans l t u.
+  Proof.
+    intros * TR.
+    now inv TR.
+  Qed.
+
+  Lemma trans_step_inv : forall l (t : ctree E B X) u,
+      trans l (Step t) u ->
+      u ≅ t /\ l = τ.
+  Proof.
+    intros * TR.
+    inv TR; split; auto.
+    rewrite <- H2. apply observe_equ_eq; auto.
+  Qed.
+
+  Lemma trans_brS_inv : forall {Y} l (c : B Y) k (u : ctree E B X),
+      trans l (BrS c k) u ->
+      exists n, u ≅ k n /\ l = τ.
+  Proof.
+    intros * TR.
+    apply trans_br_inv in TR as [n ?].
+    inv H.
+    exists n; split; auto.
+    rewrite <- H3. apply observe_equ_eq; auto.
+  Qed.
+
+  Lemma trans_stuck_inv : forall l (u : ctree E B X),
+      trans l Stuck u ->
+      False.
+  Proof.
+    intros * TR.
+    inv TR.
+  Qed.
+
+(*|
 Ad-hoc rules for pre-defined finite branching
 |*)
 
   Variable (l : @label E) (t t' u v w : ctree E B X).
-  Context `{B1 -< B} `{B2 -< B} `{B3 -< B} `{B4 -< B}.
+  Context `{B2 -< B} `{B3 -< B} `{B4 -< B}.
 
-  Lemma trans_guard_inv :
-    trans l (Guard t) t' ->
-    trans l t t'.
-  Proof.
-    intros * TR; apply trans_brD_inv in TR as [_ TR]; auto.
-  Qed.
-
-  Lemma trans_brD2_inv :
-    trans l (brD2 t u) t' ->
+  Lemma trans_br2_inv :
+    trans l (br2 t u) t' ->
     (trans l t t' \/ trans l u t').
   Proof.
-    intros * TR; apply trans_brD_inv in TR as [[] TR]; auto.
+    intros * TR; apply trans_br_inv in TR as [[] TR]; auto.
   Qed.
 
-  Lemma trans_brD3_inv :
-    trans l (brD3 t u v) t' ->
+  Lemma trans_br3_inv :
+    trans l (br3 t u v) t' ->
     (trans l t t' \/ trans l u t' \/ trans l v t').
   Proof.
-    intros * TR; apply trans_brD_inv in TR as [n TR].
+    intros * TR; apply trans_br_inv in TR as [n TR].
     destruct n; auto.
   Qed.
 
-  Lemma trans_brD4_inv :
-    trans l (brD4 t u v w) t' ->
+  Lemma trans_br4_inv :
+    trans l (br4 t u v w) t' ->
     (trans l t t' \/ trans l u t' \/ trans l v t' \/ trans l w t').
   Proof.
-    intros * TR; apply trans_brD_inv in TR as [n TR].
+    intros * TR; apply trans_br_inv in TR as [n TR].
     destruct n; auto.
-  Qed.
-
-  Lemma trans_brS_inv : forall {X} (c : B X) k,
-      trans l (BrS c k) t' ->
-      exists x, t' ≅ k x /\ l = tau.
-  Proof.
-    intros * TR.
-    cbn in *; red in TR; cbn in TR.
-    dependent induction TR.
-    eexists; split; auto.
-    rewrite H3, ctree_eta, (ctree_eta t0), x; reflexivity.
-  Qed.
-
-  Lemma trans_step_inv :
-    trans l (Step t) t' ->
-    t' ≅ t /\ l = tau.
-  Proof.
-    intros * TR; apply trans_brS_inv in TR as (_ & ? & ?); auto.
   Qed.
 
   Lemma trans_brS2_inv :
     trans l (brS2 t u) t' ->
-    (l = tau /\ (t' ≅ t \/ t' ≅ u)).
+    (l = τ /\ (t' ≅ t \/ t' ≅ u)).
   Proof.
     intros * TR; apply trans_brS_inv in TR as (? & TR & ->); split; auto.
     destruct x; auto.
@@ -760,7 +775,7 @@ Ad-hoc rules for pre-defined finite branching
 
   Lemma trans_brS3_inv :
     trans l (brS3 t u v) t' ->
-    (l = tau /\ (t' ≅ t \/ t' ≅ u \/ t' ≅ v)).
+    (l = τ /\ (t' ≅ t \/ t' ≅ u \/ t' ≅ v)).
   Proof.
     intros * TR; apply trans_brS_inv in TR as (? & TR & ->); split; auto.
     destruct x; auto.
@@ -768,13 +783,13 @@ Ad-hoc rules for pre-defined finite branching
 
   Lemma trans_brS4_inv :
     trans l (brS4 t u v w) t' ->
-    (l = tau /\ (t' ≅ t \/ t' ≅ u \/ t' ≅ v \/ t' ≅ w)).
+    (l = τ /\ (t' ≅ t \/ t' ≅ u \/ t' ≅ v \/ t' ≅ w)).
   Proof.
     intros * TR; apply trans_brS_inv in TR as (? & TR & ->); split; auto.
     destruct x; auto.
   Qed.
 
-  (*|
+(*|
 Inversion rules for [trans] based on the value of the label
 -----------------------------------------------------------
 In general, these would require to introduce the relation that
@@ -786,31 +801,30 @@ useful.
   Lemma trans__val_inv {Y} :
     forall (T U : ctree' E B X) (x : Y),
       trans_ (val x) T U ->
-      go U ≅ stuckD.
+      go U ≅ Stuck.
   Proof.
     intros * TR.
     remember (val x) as ox.
     rewrite ctree_eta; induction TR; intros; auto; try now inv Heqox.
-    step; econstructor; intros abs; inv abs.
   Qed.
 
   Lemma trans_val_inv {Y} :
     forall (t u : ctree E B X) (x : Y),
       trans (val x) t u ->
-      u ≅ stuckD.
+      u ≅ Stuck.
   Proof.
     intros * TR. cbn in TR. red in TR.
     apply trans__val_inv in TR. rewrite ctree_eta. apply TR.
   Qed.
 
   Lemma wtrans_val_inv : forall (x : X),
-      wtrans (val x) u stuckD ->
-      exists t, wtrans tau u t /\ trans (val x) t stuckD.
+      wtrans (val x) u Stuck ->
+      exists t, wtrans τ u t /\ trans (val x) t Stuck.
   Proof.
     intros * TR.
     destruct TR as [t2 [t1 step1 step2] step3].
     exists t1; split.
-    apply wtrans_tau; auto.
+    apply wtrans_τ; auto.
     erewrite <- trans_val_inv; eauto.
   Qed.
 
@@ -821,16 +835,16 @@ End forward.
 ---------------
 |*)
 
-Lemma etrans_case {E B X} `{B0 -< B} : forall l (t u : ctree E B X),
+Lemma etrans_case {E B X} : forall l (t u : ctree E B X),
     etrans l t u ->
-    (trans l t u \/ (l = tau /\ t ≅ u)).
+    (trans l t u \/ (l = τ /\ t ≅ u)).
 Proof.
   intros [] * TR; cbn in *; intuition.
 Qed.
 
-Lemma etrans_ret_inv {E B X} `{HasStuck : B0 -< B} : forall x l (t : ctree E B X),
+Lemma etrans_ret_inv {E B X} : forall x l (t : ctree E B X),
     etrans l (Ret x) t ->
-    (l = tau /\ t ≅ Ret x) \/ (l = val x /\ t ≅ stuckD).
+    (l = τ /\ t ≅ Ret x) \/ (l = val x /\ t ≅ Stuck).
 Proof.
   intros ? [] ? step; cbn in step.
   - intuition; try (eapply trans_ret in step; now apply step).
@@ -849,7 +863,7 @@ is not.
 
 Section stuck.
 
-  Context {E B : Type -> Type} {X : Type} {HasStuck: B0 -< B}.
+  Context {E B : Type -> Type} {X : Type}.
   Variable (l : @label E) (t u : ctree E B X).
 
   Definition is_stuck : ctree E B X -> Prop :=
@@ -865,7 +879,7 @@ Section stuck.
   Lemma etrans_is_stuck_inv (v v' : ctree E B X) :
     is_stuck v ->
     etrans l v v' ->
-    (l = tau /\ v ≅ v').
+    (l = τ /\ v ≅ v').
   Proof.
     intros * ST TR.
     edestruct @etrans_case; eauto.
@@ -874,7 +888,7 @@ Section stuck.
 
   Lemma transs_is_stuck_inv (v v' : ctree E B X) :
     is_stuck v ->
-    (trans tau)^* v v' ->
+    (trans τ)^* v v' ->
     v ≅ v'.
   Proof.
     intros * ST TR.
@@ -886,7 +900,7 @@ Section stuck.
   Lemma wtrans_is_stuck_inv :
     is_stuck t ->
     wtrans l t u ->
-    (l = tau /\ t ≅ u).
+    (l = τ /\ t ≅ u).
   Proof.
     intros * ST TR.
     destruct TR as [? [? ?] ?].
@@ -897,65 +911,69 @@ Section stuck.
     rewrite H, H0; auto.
   Qed.
 
-  Lemma Br0_is_stuck b (c : B void) (k : void -> _) :
-    is_stuck (Br b c k).
+  Lemma Stuck_is_stuck :
+     is_stuck Stuck.
+  Proof.
+    repeat intro; eapply trans_stuck_inv; eauto.
+  Qed.
+
+  Lemma br_void_is_stuck (c : B void) (k : void -> _) :
+    is_stuck (Br c k).
   Proof.
     red. intros. intro. inv H; destruct x.
   Qed.
 
-  Lemma Br_fin0_is_stuck b (c : B (fin 0)) (k : fin 0 -> _) :
-    is_stuck (Br b c k).
+  Lemma br_fin0_is_stuck (c : B (fin 0)) (k : fin 0 -> _) :
+    is_stuck (Br c k).
   Proof.
     red. intros. intro. inv H; now apply case0.
   Qed.
 
-  Lemma stuckD_is_stuck :
-    is_stuck stuckD.
-  Proof.
-    apply Br0_is_stuck.
-  Qed.
-
-  Lemma stuckS_is_stuck :
-    is_stuck stuckS.
-  Proof.
-    apply Br0_is_stuck.
-  Qed.
-
   Lemma spinD_gen_is_stuck {Y} (x : B Y) :
-    is_stuck (spinD_gen x).
+    is_stuck (spin_gen x).
   Proof.
     red; intros * abs.
-    remember (spinD_gen x) as v.
-    assert (EQ: v ≅ spinD_gen x) by (subst; reflexivity); clear Heqv; revert EQ; rewrite ctree_eta.
+    remember (spin_gen x) as v.
+    assert (EQ: v ≅ spin_gen x) by (subst; reflexivity); clear Heqv; revert EQ; rewrite ctree_eta.
     induction abs; auto; try now (rewrite ctree_eta; intros abs; step in abs; inv abs).
-    intros EQ; apply IHabs.
-    rewrite <- ctree_eta.
-    rewrite ctree_eta in EQ.
-    step in EQ; cbn in *.
-    dependent induction EQ; auto.
+    - intros EQ; apply IHabs.
+      rewrite <- ctree_eta.
+      rewrite ctree_eta in EQ.
+      step in EQ; cbn in *.
+      dependent induction EQ; auto.
+    - intros EQ; apply IHabs.
+      rewrite <- ctree_eta.
+      rewrite ctree_eta in EQ.
+      step in EQ; cbn in *.
+      dependent induction EQ; auto.
   Qed.
 
-  Lemma spinD_is_stuck `{B1 -< B}:
-    is_stuck spinD.
+  Lemma spin_is_stuck :
+    is_stuck spin.
   Proof.
     red; intros * abs.
-    remember spinD as v.
-    assert (EQ: v ≅ spinD) by (subst; reflexivity); clear Heqv; revert EQ; rewrite ctree_eta.
-    induction abs; auto; try now (rewrite unfold_spinD; intros abs; step in abs; inv abs).
-    intros EQ; apply IHabs.
-    rewrite <- ctree_eta.
-    rewrite unfold_spinD in EQ.
-    step in EQ.
-    dependent induction EQ; auto.
+    remember spin as v.
+    assert (EQ: v ≅ spin) by (subst; reflexivity); clear Heqv; revert EQ; rewrite ctree_eta.
+    induction abs; auto; try now (rewrite unfold_spin; intros abs; step in abs; inv abs).
+    - intros EQ; apply IHabs.
+      rewrite <- ctree_eta.
+      rewrite unfold_spin in EQ.
+      step in EQ.
+      dependent induction EQ; auto.
+    - intros EQ; apply IHabs.
+      rewrite <- ctree_eta.
+      rewrite unfold_spin in EQ.
+      step in EQ.
+      dependent induction EQ; auto.
   Qed.
 
-  Lemma spinS_is_not_stuck `{B1 -< B} :
+  Lemma spinS_is_not_stuck :
     ~ (is_stuck spinS).
   Proof.
     red; intros * abs.
-    apply (abs tau spinS).
+    apply (abs τ spinS).
     rewrite ctree_eta at 1; cbn.
-    constructor; [exact tt | reflexivity].
+    constructor; auto.
   Qed.
 
 End stuck.
@@ -967,9 +985,9 @@ wtrans theory
 
 Section wtrans.
 
-  Context {E B : Type -> Type} {X : Type} `{HasStuck : B0 -< B}.
+  Context {E B : Type -> Type} {X : Type}.
 
-  Lemma wtrans_step `{B1 -< B} : forall l (t t' : ctree E B X),
+  Lemma wtrans_step : forall l (t t' : ctree E B X),
       wtrans l t t' ->
       wtrans l (Step t) t'.
   Proof.
@@ -978,8 +996,8 @@ Section wtrans.
     apply trans_step.
   Qed.
 
-  Lemma trans_tau_str_ret_inv : forall x (t : ctree E B X),
-      (trans tau)^* (Ret x) t ->
+  Lemma trans_τ_str_ret_inv : forall x (t : ctree E B X),
+      (trans τ)^* (Ret x) t ->
       t ≅ Ret x.
   Proof.
     intros * [[|] step].
@@ -990,30 +1008,30 @@ Section wtrans.
 
   Lemma wtrans_ret_inv : forall x l (t : ctree E B X),
       wtrans l (Ret x) t ->
-      (l = tau /\ t ≅ Ret x) \/ (l = val x /\ t ≅ stuckD).
+      (l = τ /\ t ≅ Ret x) \/ (l = val x /\ t ≅ Stuck).
   Proof.
     intros * step.
     destruct step as [? [? step1 step2] step3].
-    apply trans_tau_str_ret_inv in step1.
+    apply trans_τ_str_ret_inv in step1.
     rewrite step1 in step2; clear step1.
     apply etrans_ret_inv in step2 as [[-> EQ] |[-> EQ]].
-    rewrite EQ in step3; apply trans_tau_str_ret_inv in step3; auto.
+    rewrite EQ in step3; apply trans_τ_str_ret_inv in step3; auto.
     rewrite EQ in step3.
-    apply transs_is_stuck_inv in step3; [| apply stuckD_is_stuck].
+    apply transs_is_stuck_inv in step3; [| apply Stuck_is_stuck].
     intuition.
   Qed.
 
   Lemma wtrans_val_inv' : forall (x : X) (t v : ctree E B X),
       wtrans (val x) t v ->
-      exists u, wtrans tau t u /\ trans (val x) u v /\ v ≅ stuckD.
+      exists u, wtrans τ t u /\ trans (val x) u v /\ v ≅ Stuck.
   Proof.
     intros * TR.
     destruct TR as [t2 [t1 step1 step2] step3].
     pose proof trans_val_inv step2 as EQ.
     rewrite EQ in step3, step2.
-    apply transs_is_stuck_inv in step3; auto using stuckD_is_stuck.
+    apply transs_is_stuck_inv in step3; auto using Stuck_is_stuck.
     exists t1; repeat split.
-    apply wtrans_tau, step1.
+    apply wtrans_τ, step1.
     rewrite <- step3; auto.
     symmetry; auto.
   Qed.
@@ -1027,79 +1045,85 @@ trans l (t >>= k) u -> (trans l t t' /\ u ≅ t' >>= k) \/ (trans (ret x) t stuc
 l <> val x -> trans l t u -> trans l (t >>= k) (u >>= k)
 trans (val x) t stuck -> trans l (k x) u -> trans l (bind t k) u.
 |*)
-Lemma trans_bind_inv_aux {E B X Y} `{HasStuck : B0 -< B} l T U :
+Lemma trans_bind_inv_aux {E B X Y} l T U :
   trans_ l T U ->
   forall (t : ctree E B X) (k : X -> ctree E B Y) (u : ctree E B Y),
     go T ≅ t >>= k ->
     go U ≅ u ->
     (~ (is_val l) /\ exists t', trans l t t' /\ u ≅ t' >>= k) \/
-      (exists (x : X), trans (val x) t stuckD /\ trans l (k x) u).
+      (exists (x : X), trans (val x) t Stuck /\ trans l (k x) u).
 Proof.
   intros TR; induction TR; intros.
+
   - rewrite unfold_bind in H; setoid_rewrite (ctree_eta t0).
     desobs t0.
     + right.
       exists r; split.
       constructor.
       rewrite <- H.
-      apply (Stepbr _ x); auto.
+      apply (Transbr _ x); auto.
       rewrite <- H0; auto.
     + step in H; inv H.
+    + step in H; dependent induction H.
+    + step in H; dependent induction H.
+    + step in H; dependent induction H.
     + step in H; dependent induction H.
       specialize (IHTR (k1 x) k0 u).
       destruct IHTR as [(? & ? & ? & ?) | (? & ? & ?)]; auto.
       rewrite <- ctree_eta, REL; reflexivity.
       left; split; eauto.
       exists x0; split; auto.
-      apply (Stepbr _ x); auto.
+      apply (Transbr _ x); auto.
       right.
       exists x0; split; auto.
-      apply (Stepbr _ x); auto.
-  - rewrite unfold_bind in H0; setoid_rewrite (ctree_eta t0).
-    desobs t0.
+      apply (Transbr _ x); auto.
+
+  - symmetry in H; apply guard_equ_bind in H.
+    destruct H as [(? & EQ & EQ') | (? & EQ & EQ')].
     + right.
-      exists r; split.
-      constructor.
-      rewrite <- H0.
-      apply (Steptau _ x); auto.
-      rewrite H, <- H1, ctree_eta; auto.
-    + step in H0; inv H0.
-    + step in H0; dependent induction H0.
-      left; split; [intros abs; inv abs |].
-      exists (k1 x); split.
-      econstructor; reflexivity.
-      rewrite <- H1, <- ctree_eta, <- H.
-      apply REL.
-  - rewrite unfold_bind in H0; setoid_rewrite (ctree_eta t0).
-    desobs t0.
+      exists x; split; [rewrite EQ; constructor |].
+      rewrite EQ'; auto.
+      rewrite <- H0; constructor; auto.
+    + destruct (IHTR x k u).
+      rewrite EQ', <- ctree_eta; auto.
+      auto.
+      destruct H as (?& (? & ? & ?)); left; split; eauto.
+      eexists; split.
+      rewrite EQ; constructor; apply H1.
+      auto.
+      destruct H as (? & ? & ?).
+      right; eexists; split; eauto.
+      rewrite EQ; constructor.
+      apply H.
+  - symmetry in H0; apply step_equ_bind in H0.
+    destruct H0 as [(? & EQ & EQ') | (? & EQ & EQ')].
     + right.
-      exists r; split.
-      constructor.
-      rewrite <- H0.
-      constructor.
-      rewrite H, <- H1, ctree_eta; auto.
-    + step in H0; dependent induction H0.
-      left; split; [intros abs; inv abs |].
-      exists (k1 x); split.
-      econstructor; reflexivity.
-      rewrite <- H1, <- ctree_eta, <- H.
-      apply REL.
-    + step in H0; inv H0.
-  - rewrite unfold_bind in H; setoid_rewrite (ctree_eta t).
-    desobs t.
+      exists x; split; [rewrite EQ; constructor |].
+      rewrite EQ'; constructor.
+      rewrite <- ctree_eta in H1; rewrite <- H1; auto.
+    + left; split; [apply is_val_τ |].
+      eexists; split; [rewrite EQ; constructor; reflexivity |].
+      rewrite <- H1, <- ctree_eta, H, <-EQ'; auto.
+  - symmetry in H0; apply vis_equ_bind in H0.
+    destruct H0 as [(? & EQ & EQ') | (? & EQ & EQ')].
     + right.
-      exists r0; split.
-      constructor.
-      rewrite <- H, <- H0.
-      constructor.
-    + step in H; inv H.
-    + step in H; inv H.
+      exists x0; split; [rewrite EQ; constructor |].
+      rewrite EQ'; constructor.
+      rewrite <- ctree_eta in H1; rewrite <- H1; auto.
+    + left; split; [apply is_val_obs |].
+      eexists; split; [rewrite EQ; constructor; reflexivity |].
+      rewrite <- H1, <- ctree_eta, <- H, <-EQ'; auto.
+  - symmetry in H; apply ret_equ_bind in H.
+    destruct H as (? & EQ & EQ').
+    right.
+    exists x; split; [rewrite EQ; constructor |].
+    rewrite EQ', <- H0; econstructor.
 Qed.
 
-Lemma trans_bind_inv {E B X Y} `{B0 -< B} (t : ctree E B X) (k : X -> ctree E B Y) (u : ctree E B Y) l :
+Lemma trans_bind_inv {E B X Y} (t : ctree E B X) (k : X -> ctree E B Y) (u : ctree E B Y) l :
   trans l (t >>= k) u ->
   (~ (is_val l) /\ exists t', trans l t t' /\ u ≅ t' >>= k) \/
-    (exists (x : X), trans (val x) t stuckD /\ trans l (k x) u).
+    (exists (x : X), trans (val x) t Stuck /\ trans l (k x) u).
 Proof.
   intros TR.
   eapply trans_bind_inv_aux.
@@ -1108,7 +1132,7 @@ Proof.
   rewrite <- ctree_eta; reflexivity.
 Qed.
 
-Lemma trans_bind_inv_l {E B X Y} `{B0 -< B} (t : ctree E B X) (k : X -> ctree E B Y) (u : ctree E B Y) l :
+Lemma trans_bind_inv_l {E B X Y} (t : ctree E B X) (k : X -> ctree E B Y) (u : ctree E B Y) l :
   trans l (t >>= k) u ->
   exists l' t', trans l' t t'.
 Proof.
@@ -1117,7 +1141,7 @@ Proof.
   destruct TR as [(? & ? & ? & ?) | (? & ? & ?)]; eauto.
 Qed.
 
-Lemma trans_bind_l {E B X Y} `{HasStuck : B0 -< B} (t : ctree E B X) (k : X -> ctree E B Y) (u : ctree E B X) l :
+Lemma trans_bind_l {E B X Y} (t : ctree E B X) (k : X -> ctree E B Y) (u : ctree E B X) l :
   ~ (@is_val E l) ->
   trans l t u ->
   trans l (t >>= k) (u >>= k).
@@ -1128,12 +1152,13 @@ Proof.
     cbn.
     econstructor.
     now apply IHTR.
+  - rewrite unfold_bind, <- x; cbn.
+    constructor.
+    apply IHTR; auto.
   - rewrite unfold_bind.
-    rewrite <- x1; cbn.
+    rewrite <- x0; cbn.
     econstructor.
-    rewrite H.
-    rewrite (ctree_eta t0),x,<- ctree_eta.
-    reflexivity.
+    now rewrite <- H, (ctree_eta u0), x, <- ctree_eta.
   - rewrite unfold_bind.
     rewrite <- x1; cbn.
     econstructor.
@@ -1143,33 +1168,36 @@ Proof.
   - exfalso; eapply NOV; constructor.
 Qed.
 
-Lemma trans_bind_r {E B X Y} `{B0 -< B} (t : ctree E B X) (k : X -> ctree E B Y) (u : ctree E B Y) x l :
-  trans (val x) t stuckD ->
+Lemma trans_bind_r {E B X Y} (t : ctree E B X) (k : X -> ctree E B Y) (u : ctree E B Y) x l :
+  trans (val x) t Stuck ->
   trans l (k x) u ->
   trans l (t >>= k) u.
 Proof.
   cbn; unfold transR; intros TR1.
   genobs t ot.
-  remember (observe stuckD) as oc.
+  remember (observe Stuck) as oc.
   remember (val x) as v.
   revert t x Heqot Heqoc Heqv.
   induction TR1; intros; try (inv Heqv; fail).
+  - subst.
+    rewrite (ctree_eta t0), <- Heqot; cbn; econstructor.
+    eapply IHTR1; eauto.
   - rewrite (ctree_eta t0), <- Heqot; cbn; econstructor.
     eapply IHTR1; eauto.
   - dependent induction Heqv.
     rewrite (ctree_eta t), <- Heqot, unfold_bind; cbn; auto.
 Qed.
 
-Lemma is_stuck_bind : forall {E B X Y} `{B0 -< B}
+Lemma is_stuck_bind : forall {E B X Y}
                         (t : ctree E B X) (k : X -> ctree E B Y),
     is_stuck t -> is_stuck (bind t k).
 Proof.
   repeat intro.
-  apply trans_bind_inv in H1 as [].
-  - destruct H1 as (? & ? & ? & ?).
-    now apply H0 in H2.
-  - destruct H1 as (? & ? & ?).
-    now apply H0 in H1.
+  apply trans_bind_inv in H0 as [].
+  - destruct H0 as (? & ? & ? & ?).
+    now apply H in H1.
+  - destruct H0 as (? & ? & ?).
+    now apply H in H0.
 Qed.
 
 (*|
@@ -1177,10 +1205,10 @@ Forward and backward rules for [wtrans] w.r.t. [bind]
 -----------------------------------------------------
 |*)
 
-Lemma etrans_bind_inv {E B X Y} `{HasStuck : B0 -< B} (t : ctree E B X) (k : X -> ctree E B Y) (u : ctree E B Y) l :
+Lemma etrans_bind_inv {E B X Y} (t : ctree E B X) (k : X -> ctree E B Y) (u : ctree E B Y) l :
   etrans l (t >>= k) u ->
   (~ (is_val l) /\ exists t', etrans l t t' /\ u ≅ t' >>= k) \/
-    (exists (x : X), trans (val x) t stuckD /\ etrans l (k x) u).
+    (exists (x : X), trans (val x) t Stuck /\ etrans l (k x) u).
 Proof.
   intros TR.
   apply @etrans_case in TR as [ | (-> & ?)].
@@ -1193,10 +1221,10 @@ Proof.
     exists t; split; auto using enil; symmetry; auto.
 Qed.
 
-Lemma transs_bind_inv {E B X Y} `{B0 -< B} (t : ctree E B X) (k : X -> ctree E B Y) (u : ctree E B Y) :
-  (trans tau)^* (t >>= k) u ->
-  (exists t', (trans tau)^* t t' /\ u ≅ t' >>= k) \/
-    (exists (x : X), wtrans (val x) t stuckD /\ (trans tau)^* (k x) u).
+Lemma transs_bind_inv {E B X Y} (t : ctree E B X) (k : X -> ctree E B Y) (u : ctree E B Y) :
+  (trans τ)^* (t >>= k) u ->
+  (exists t', (trans τ)^* t t' /\ u ≅ t' >>= k) \/
+    (exists (x : X), wtrans (val x) t Stuck /\ (trans τ)^* (k x) u).
 Proof.
   intros [n TR].
   revert t k u TR.
@@ -1210,8 +1238,8 @@ Proof.
     + rewrite EQ in TR2; clear t1 EQ.
       apply IH in TR2 as [(t3 & TR2 & EQ')| (x & TR2 & TR3)].
       * left; eexists; split; eauto.
-        apply wtrans_tau; eapply wcons; eauto.
-        apply wtrans_tau; auto.
+        apply wtrans_τ; eapply wcons; eauto.
+        apply wtrans_τ; auto.
       * right; exists x; split; eauto.
         eapply wcons; eauto.
     + right.
@@ -1231,11 +1259,11 @@ in the prefix. This is a bit more annoying to express: we cannot necessarily
 just before the [Ret] some invisible br nodes. We therefore have to introduce
 the last visible state reached by [wtrans] and add a [trans (val _)] afterward.
 |*)
-Lemma wtrans_bind_inv {E B X Y} `{HasStuck : B0 -< B} (t : ctree E B X) (k : X -> ctree E B Y) (u : ctree E B Y) l :
+Lemma wtrans_bind_inv {E B X Y} (t : ctree E B X) (k : X -> ctree E B Y) (u : ctree E B Y) l :
   wtrans l (t >>= k) u ->
   (~ (is_val l) /\ exists t', wtrans l t t' /\ u ≅ t' >>= k) \/
-    (exists (x : X), wtrans (val x) t stuckD /\ wtrans l (k x) u) \/
-    (exists (x : X) s, wtrans l t s /\ trans (val x) s stuckD /\ wtrans tau (k x) u).
+    (exists (x : X), wtrans (val x) t Stuck /\ wtrans l (k x) u) \/
+    (exists (x : X) s, wtrans l t s /\ trans (val x) s Stuck /\ wtrans τ (k x) u).
 Proof.
   intros TR.
   destruct TR as [t2 [t1 step1 step2] step3].
@@ -1251,20 +1279,20 @@ Proof.
         apply wtrans_val_inv in TR3 as (u3 & TR2' & TR2'').
         exists x, u3.
         split; [|split]; auto.
-        2:apply wtrans_tau; auto.
+        2:apply wtrans_τ; auto.
         exists u2; [exists u1; assumption | ].
-        apply wtrans_tau; apply wtrans_tau in TR1.
+        apply wtrans_τ; apply wtrans_τ in TR1.
         eapply wconss; eauto.
     + right; left.
       exists x; split.
-      eexists; [eexists |]; eauto; apply wtrans_tau, wnil.
-      eexists; [eexists |]; eauto; apply wtrans_tau, wnil.
+      eexists; [eexists |]; eauto; apply wtrans_τ, wnil.
+      eexists; [eexists |]; eauto; apply wtrans_τ, wnil.
   - right; left.
     exists x; split; eauto.
     eexists; [eexists |]; eauto.
 Qed.
 
-Lemma etrans_bind_l {E B X Y} `{B0 -< B} (t : ctree E B X) (k : X -> ctree E B Y) (u : ctree E B X) l :
+Lemma etrans_bind_l {E B X Y} (t : ctree E B X) (k : X -> ctree E B Y) (u : ctree E B X) l :
   ~ is_val l ->
   etrans l t u ->
   etrans l (t >>= k) (u >>= k).
@@ -1272,12 +1300,12 @@ Proof.
   destruct l; cbn; try apply trans_bind_l; auto.
   intros NOV [|].
   left; apply trans_bind_l; auto.
-  right; rewrite H0; auto.
+  right; rewrite H; auto.
 Qed.
 
-Lemma transs_bind_l {E B X Y} `{B0 -< B} (t : ctree E B X) (k : X -> ctree E B Y) (u : ctree E B X) :
-  (trans tau)^* t u ->
-  (trans tau)^* (t >>= k) (u >>= k).
+Lemma transs_bind_l {E B X Y} (t : ctree E B X) (k : X -> ctree E B Y) (u : ctree E B X) :
+  (trans τ)^* t u ->
+  (trans τ)^* (t >>= k) (u >>= k).
 Proof.
   intros [n TR].
   revert t u TR.
@@ -1285,12 +1313,12 @@ Proof.
   - cbn; intros; exists 0%nat; cbn; rewrite TR; reflexivity.
   - intros t u [v TR1 TR2].
     apply IH in TR2.
-    eapply wtrans_tau, wcons.
+    eapply wtrans_τ, wcons.
     apply trans_bind_l; eauto; intros abs; inv abs.
-    apply wtrans_tau; eauto.
+    apply wtrans_τ; eauto.
 Qed.
 
-Lemma wtrans_bind_l {E B X Y} `{B0 -< B} (t : ctree E B X) (k : X -> ctree E B Y) (u : ctree E B X) l :
+Lemma wtrans_bind_l {E B X Y} (t : ctree E B X) (k : X -> ctree E B Y) (u : ctree E B X) l :
   ~ (@is_val E l) ->
   wtrans l t u ->
   wtrans l (t >>= k) (u >>= k).
@@ -1302,21 +1330,21 @@ Proof.
   apply transs_bind_l; eauto.
 Qed.
 
-Lemma wtrans_case {E B X} `{HasStuck : B0 -< B} (t u : ctree E B X) l:
+Lemma wtrans_case {E B X} (t u : ctree E B X) l:
   wtrans l t u ->
-  t ≅ u \/ (exists v, trans l t v /\ wtrans tau v u) \/ (exists v, trans tau t v /\ wtrans l v u).
+  t ≅ u \/ (exists v, trans l t v /\ wtrans τ v u) \/ (exists v, trans τ t v /\ wtrans l v u).
 Proof.
   intros [t2 [t1 [n TR1] TR2] TR3].
   destruct n as [| n].
-  - apply wtrans_tau in TR3.
+  - apply wtrans_τ in TR3.
     cbn in TR1; rewrite <- TR1 in TR2.
     destruct l; eauto.
     destruct TR2; eauto.
     cbn in H; rewrite <- H in TR3.
-    apply wtrans_tau in TR3.
+    apply wtrans_τ in TR3.
     destruct TR3 as [[| n] ?]; eauto.
     destruct H0 as [? ? ?]; right; left; eexists; split; eauto.
-    apply wtrans_tau; exists n; auto.
+    apply wtrans_τ; exists n; auto.
   - destruct TR1 as [? ? ?].
     right; right.
     eexists; split; eauto.
@@ -1324,25 +1352,25 @@ Proof.
     exists n; eauto.
 Qed.
 
-Lemma wtrans_case' {E B X} `{HasStuck : B0 -< B} (t u : ctree E B X) l:
+Lemma wtrans_case' {E B X} (t u : ctree E B X) l:
   wtrans l t u ->
   match l with
-  | tau => (t ≅ u \/ exists v, trans tau t v /\ wtrans tau v u)
-  | _   => (exists v, trans l t v /\ wtrans tau v u) \/
-            (exists v, trans tau t v /\ wtrans l v u)
+  | τ => (t ≅ u \/ exists v, trans τ t v /\ wtrans τ v u)
+  | _   => (exists v, trans l t v /\ wtrans τ v u) \/
+            (exists v, trans τ t v /\ wtrans l v u)
   end.
 Proof.
   intros [t2 [t1 [n TR1] TR2] TR3].
   destruct n as [| n].
-  - apply wtrans_tau in TR3.
+  - apply wtrans_τ in TR3.
     cbn in TR1; rewrite <- TR1 in TR2.
     destruct l; eauto.
     destruct TR2; eauto.
     cbn in H; rewrite <- H in TR3.
-    apply wtrans_tau in TR3.
+    apply wtrans_τ in TR3.
     destruct TR3 as [[| n] ?]; eauto.
     destruct H0 as [? ? ?]; right; eexists; split; eauto.
-    apply wtrans_tau; exists n; auto.
+    apply wtrans_τ; exists n; auto.
   - destruct TR1 as [? ? ?].
     destruct l; right.
     all:eexists; split; eauto.
@@ -1350,25 +1378,25 @@ Proof.
           all:exists n; eauto.
 Qed.
 
-Lemma wtrans_stuckD_inv {E B R} `{HasStuck : B0 -< B} :
+Lemma wtrans_Stuck_inv {E B R} :
   forall (t : ctree E B R) l,
-    wtrans l stuckD t ->
-    match l with | tau => t ≅ stuckD | _ => False end.
+    wtrans l Stuck t ->
+    match l with | τ => t ≅ Stuck | _ => False end.
 Proof.
   intros * TR.
   apply wtrans_case' in TR.
   destruct l; break; cbn in *.
   symmetry; auto.
-  all: exfalso; eapply stuckD_is_stuck; now apply H.
+  all: exfalso; eapply Stuck_is_stuck; now apply H.
 Qed.
 
-Lemma pwtrans_case {E B X} `{B0 -< B} (t u : ctree E B X) l:
+Lemma pwtrans_case {E B X} (t u : ctree E B X) l:
   pwtrans l t u ->
-  (exists v, trans l t v /\ wtrans tau v u) \/ (exists v, trans tau t v /\ wtrans l v u).
+  (exists v, trans l t v /\ wtrans τ v u) \/ (exists v, trans τ t v /\ wtrans l v u).
 Proof.
   intros [t2 [t1 [n TR1] TR2] TR3].
   destruct n as [| n].
-  - apply wtrans_tau in TR3.
+  - apply wtrans_τ in TR3.
     cbn in TR1; rewrite <- TR1 in TR2. eauto.
   - destruct TR1 as [? ? ?].
     right.
@@ -1384,8 +1412,8 @@ It's a bit annoying that we need two cases in this lemma, but if
 by taking the [Ret] in the prefix, but we cannot process it to
 reach [u] in the bound computation.
 |*)
-Lemma wtrans_bind_r {E B X Y} `{HasStuck : B0 -< B} (t : ctree E B X) (k : X -> ctree E B Y) (u : ctree E B Y) x l :
-  wtrans (val x) t stuckD ->
+Lemma wtrans_bind_r {E B X Y} (t : ctree E B X) (k : X -> ctree E B Y) (u : ctree E B Y) x l :
+  wtrans (val x) t Stuck ->
   wtrans l (k x) u ->
   (u ≅ k x \/ wtrans l (t >>= k) u).
 Proof.
@@ -1406,8 +1434,8 @@ Proof.
     apply trans_wtrans; auto.
 Qed.
 
-Lemma wtrans_bind_r' {E B X Y} `{HasStuck : B0 -< B} (t : ctree E B X) (k : X -> ctree E B Y) (u : ctree E B Y) x l :
-  wtrans (val x) t stuckD ->
+Lemma wtrans_bind_r' {E B X Y} (t : ctree E B X) (k : X -> ctree E B Y) (u : ctree E B Y) x l :
+  wtrans (val x) t Stuck ->
   pwtrans l (k x) u ->
   (wtrans l (t >>= k) u).
 Proof.
@@ -1427,7 +1455,7 @@ Proof.
     apply trans_wtrans; auto.
 Qed.
 
-Lemma trans_val_invT {E B R R'} `{B0 -< B}:
+Lemma trans_val_invT {E B R R'} :
   forall (t u : ctree E B R) (v : R'),
     trans (val v) t u ->
     R = R'.
@@ -1437,10 +1465,10 @@ Proof.
   induction TR; intros; auto; try now inv Heqov.
 Qed.
 
-Lemma wtrans_bind_lr {E B X Y} `{B0 -< B} (t u : ctree E B X) (k : X -> ctree E B Y) (v : ctree E B Y) x l :
+Lemma wtrans_bind_lr {E B X Y} (t u : ctree E B X) (k : X -> ctree E B Y) (v : ctree E B Y) x l :
   pwtrans l t u ->
-  wtrans (val x) u stuckD ->
-  pwtrans tau (k x) v ->
+  wtrans (val x) u Stuck ->
+  pwtrans τ (k x) v ->
   (wtrans l (t >>= k) v).
 Proof.
   intros [t2 [t1 TR1 TR1'] TR1''] TR2 TR3.
@@ -1452,21 +1480,21 @@ Proof.
       pose proof (trans_val_invT TR1'); subst.
       apply trans_val_inv in TR1'.
       rewrite TR1' in TR1''.
-      apply transs_is_stuck_inv in TR1''; [| apply stuckD_is_stuck].
+      apply transs_is_stuck_inv in TR1''; [| apply Stuck_is_stuck].
       rewrite <- TR1'' in TR2.
-      apply wtrans_is_stuck_inv in TR2; [| apply stuckD_is_stuck].
+      apply wtrans_is_stuck_inv in TR2; [| apply Stuck_is_stuck].
       destruct TR2 as [abs _]; inv abs.
     }
     eexists.
     2:apply trans_etrans, trans_bind_l; eauto.
-    apply wtrans_tau; eapply wtrans_bind_l; [intros abs; inv abs| apply wtrans_tau; auto].
-  - apply wtrans_tau.
+    apply wtrans_τ; eapply wtrans_bind_l; [intros abs; inv abs| apply wtrans_τ; auto].
+  - apply wtrans_τ.
     eapply wconss.
-    eapply wtrans_bind_l; [intros abs; inv abs| apply wtrans_tau; eauto].
+    eapply wtrans_bind_l; [intros abs; inv abs| apply wtrans_τ; eauto].
     eapply wtrans_bind_r'; eauto.
 Qed.
 
-Lemma trans_trigger : forall {E B X Y} `{B0 -< B} (e : E X) x (k : X -> ctree E B Y),
+Lemma trans_trigger : forall {E B X Y} (e : E X) x (k : X -> ctree E B Y),
     trans (obs e x) (trigger e >>= k) (k x).
 Proof.
   intros.
@@ -1476,7 +1504,7 @@ Proof.
   constructor; auto.
 Qed.
 
-Lemma trans_trigger' : forall {E B X Y} `{B0 -< B} (e : E X) x (t : ctree E B Y),
+Lemma trans_trigger' : forall {E B X Y} (e : E X) x (t : ctree E B Y),
     trans (obs e x) (trigger e;; t) t.
 Proof.
   intros.
@@ -1486,7 +1514,7 @@ Proof.
   constructor; auto.
 Qed.
 
-Lemma trans_trigger_inv : forall {E B X Y} `{HasStuck : B0 -< B} (e : E X) (k : X -> ctree E B Y) l u,
+Lemma trans_trigger_inv : forall {E B X Y} (e : E X) (k : X -> ctree E B Y) l u,
     trans l (trigger e >>= k) u ->
     exists x, u ≅ k x /\ l = obs e x.
 Proof.
@@ -1502,13 +1530,13 @@ Proof.
 Qed.
 
 Lemma trans_branch :
-  forall {E B : Type -> Type} {X : Type} {H : B0 -< B} {Y : Type}
+  forall {E B : Type -> Type} {X : Type} {Y : Type}
     [l : label] [t t' : ctree E B X] (c : B Y) (k : Y -> ctree E B X) (x : Y),
-    trans l t t' -> k x ≅ t -> trans l (CTree.branch false c >>= k) t'.
+    trans l t t' -> k x ≅ t -> trans l (branch c >>= k) t'.
 Proof.
   intros.
   setoid_rewrite bind_branch.
-  eapply trans_brD; eauto.
+  eapply trans_br; eauto.
 Qed.
 
 (*|
@@ -1527,11 +1555,11 @@ Proof.
   red. intros. subst. exfalso. apply H. constructor.
 Qed.
 
-Lemma wf_val_trans {E B X} `{B0 -< B} (l : @label E) (t t' : ctree E B X) :
+Lemma wf_val_trans {E B X} (l : @label E) (t t' : ctree E B X) :
   trans l t t' -> wf_val X l.
 Proof.
   red. intros. subst.
-  now apply trans_val_invT in H0.
+  now apply trans_val_invT in H.
 Qed.
 
 Lemma wf_val_is_val_inv : forall {E} X (l : @label E),
@@ -1544,17 +1572,17 @@ Proof.
   specialize (H0 X0 x eq_refl). subst. eauto.
 Qed.
 
-(*| If the LTS has events of type [L +' R] then 
+(*| If the LTS has events of type [L +' R] then
   it is possible to step it as either an [L] LTS
   or [R] LTS ignoring the other.
- |*)
+*)
 Section Coproduct.
   Arguments label: clear implicits.
-  Context {L R C: Type -> Type} {X: Type} {HasStuck: B0 -< C}.
+  Context {L R C: Type -> Type} {X: Type}.
   Notation S := (ctree (L +' R) C X).
   Notation S' := (ctree' (L +' R) C X).
   Notation SP := (SS -> label (L +' R) -> Prop).
-    
+
   (* Skip an [R] event *)
   Inductive srtrans_: rel S' S' :=
   | IgnoreR {X} (e : R X) k x t :
@@ -1578,14 +1606,14 @@ Section Coproduct.
     {| hrel_of := (fun (u v: SS) => sltrans_ (observe u) (observe v)) |}.
   Next Obligation. split; induction 1; auto. Defined.
 
-  (*| Obs transition on the left, ignores right transitions and [tau] |*)
-  Definition ltrans {X}(l: L X)(x: X): srel SS SS := 
-    (trans tau ⊔ srtrans)^* ⋅ trans (obs (inl1 l) x) ⋅ (trans tau ⊔ srtrans)^*.
+  (*| Obs transition on the left, ignores right transitions and [τ] |*)
+  Definition ltrans {X}(l: L X)(x: X): srel SS SS :=
+    (trans τ ⊔ srtrans)^* ⋅ trans (obs (inl1 l) x) ⋅ (trans τ ⊔ srtrans)^*.
 
-  (*| Obs transition on the right, ignores left transitions and [tau] |*)
-  Definition rtrans {X}(r: R X)(x: X): srel SS SS := 
-    (trans tau ⊔ sltrans)^* ⋅ trans (obs (inr1 r) x) ⋅ (trans tau ⊔ sltrans)^*.
-  
+  (*| Obs transition on the right, ignores left transitions and [τ] |*)
+  Definition rtrans {X}(r: R X)(x: X): srel SS SS :=
+    (trans τ ⊔ sltrans)^* ⋅ trans (obs (inr1 r) x) ⋅ (trans τ ⊔ sltrans)^*.
+
 End Coproduct.
 
 (*|
@@ -1604,7 +1632,7 @@ Ltac inv_trans_one :=
       apply trans_ret_inv in h as [?EQ EQl];
       match type of EQl with
       | val _   = val _ => apply val_eq_inv in EQl; try (inversion EQl; fail)
-      | tau     = val _ => now inv EQl
+      | τ     = val _ => now inv EQl
       | obs _ _ = val _ => now inv EQl
       | _ => idtac
       end
@@ -1623,7 +1651,7 @@ Ltac inv_trans_one :=
           apply obs_eq_inv in EQl as [EQe EQv];
           try (inversion EQv; inversion EQe; fail)
       | val _   = obs _ _ => now inv EQl
-      | tau     = obs _ _ => now inv EQl
+      | τ     = obs _ _ => now inv EQl
       | _ => idtac
       end
 
@@ -1632,9 +1660,9 @@ Ltac inv_trans_one :=
       let EQl := fresh "EQl" in
       apply trans_step_inv in h as (?EQ & EQl);
       match type of EQl with
-      | tau     = tau => clear EQl
-      | val _   = tau => now inv EQl
-      | obs _ _ = tau => now inv EQl
+      | τ     = τ => clear EQl
+      | val _   = τ => now inv EQl
+      | obs _ _ = τ => now inv EQl
       | _ => idtac
       end
 
@@ -1644,9 +1672,9 @@ Ltac inv_trans_one :=
       let EQl := fresh "EQl" in
       apply trans_brS_inv in h as (x & ?EQ & EQl);
       match type of EQl with
-      | tau     = tau => clear EQl
-      | val _   = tau => now inv EQl
-      | obs _ _ = tau => now inv EQl
+      | τ     = τ => clear EQl
+      | val _   = τ => now inv EQl
+      | obs _ _ = τ => now inv EQl
       | _ => idtac
       end
 
@@ -1655,9 +1683,9 @@ Ltac inv_trans_one :=
       let EQl := fresh "EQl" in
       apply trans_brS2_inv in h as (EQl & [?EQ | ?EQ]);
       match type of EQl with
-      | tau     = tau => clear EQl
-      | val _   = tau => now inv EQl
-      | obs _ _ = tau => now inv EQl
+      | τ     = τ => clear EQl
+      | val _   = τ => now inv EQl
+      | obs _ _ = τ => now inv EQl
       | _ => idtac
       end
 
@@ -1666,9 +1694,9 @@ Ltac inv_trans_one :=
       let EQl := fresh "EQl" in
       apply trans_brS3_inv in h as (EQl & [?EQ | [?EQ | ?EQ]]);
       match type of EQl with
-      | tau     = tau => clear EQl
-      | val _   = tau => now inv EQl
-      | obs _ _ = tau => now inv EQl
+      | τ     = τ => clear EQl
+      | val _   = τ => now inv EQl
+      | obs _ _ = τ => now inv EQl
       | _ => idtac
       end
 
@@ -1677,9 +1705,9 @@ Ltac inv_trans_one :=
       let EQl := fresh "EQl" in
       apply trans_brS4_inv in h as (EQl & [?EQ | [?EQ | [?EQ | ?EQ]]]);
       match type of EQl with
-      | tau     = tau => clear EQl
-      | val _   = tau => now inv EQl
-      | obs _ _ = tau => now inv EQl
+      | τ     = τ => clear EQl
+      | val _   = τ => now inv EQl
+      | obs _ _ = τ => now inv EQl
       | _ => idtac
       end
 
@@ -1687,29 +1715,29 @@ Ltac inv_trans_one :=
   | h : trans' _ (Guard _) _ |- _ =>
       apply trans_guard_inv in h
 
-  (* BrD *)
-  | h : trans' _ (BrD ?n ?k) _ |- _ =>
+  (* Br *)
+  | h : trans' _ (Br ?n ?k) _ |- _ =>
       let x := fresh "x" in
-      apply trans_brD_inv in h as (x & ?TR)
+      apply trans_br_inv in h as (x & ?TR)
 
-  (* brD2 *)
-  | h : trans' _ (brD2 _ _) _ |- _ =>
-      apply trans_brD2_inv in h as [?TR | ?TR]
+  (* br2 *)
+  | h : trans' _ (br2 _ _) _ |- _ =>
+      apply trans_br2_inv in h as [?TR | ?TR]
 
-  (* brD3 *)
-  | h : trans' _ (brD3 _ _ _) _ |- _ =>
-      apply trans_brD3_inv in h as [?TR | [?TR | ?TR]]
+  (* br3 *)
+  | h : trans' _ (br3 _ _ _) _ |- _ =>
+      apply trans_br3_inv in h as [?TR | [?TR | ?TR]]
 
-  (* brD4 *)
-  | h : trans' _ (brD4 _ _ _ _) _ |- _ =>
-      apply trans_brD4_inv in h as [?TR | [?TR | [?TR | ?TR]]]
+  (* br4 *)
+  | h : trans' _ (br4 _ _ _ _) _ |- _ =>
+      apply trans_br4_inv in h as [?TR | [?TR | [?TR | ?TR]]]
 
-  (* stuckD *)
-  | h : trans' _ stuckD _ |- _ =>
-      exfalso; eapply stuckD_is_stuck; now apply h
-  (* stuckS *)
-  | h : trans' _ stuckS _ |- _ =>
-      exfalso; eapply stuckS_is_stuck; now apply h
+  (* Stuck *)
+  | h : trans' _ Stuck _ |- _ =>
+      exfalso; eapply Stuck_is_stuck; now apply h
+  (* (* stuckS *) *)
+  (* | h : trans' _ stuckS _ |- _ => *)
+  (*     exfalso; eapply stuckS_is_stuck; now apply h *)
 
   (* trigger *)
   | h : trans' _ (CTree.bind (CTree.trigger ?e) ?t) _ |- _ =>
@@ -1722,11 +1750,11 @@ Ltac inv_trans := repeat inv_trans_one.
 
 Create HintDb trans.
 #[global] Hint Resolve
- trans_ret trans_vis trans_brS trans_brD
+ trans_ret trans_vis trans_brS trans_br
  trans_guard
- trans_brD21 trans_brD22
- trans_brD31 trans_brD32 trans_brD33
- trans_brD41 trans_brD42 trans_brD43 trans_brD44
+ trans_br21 trans_br22
+ trans_br31 trans_br32 trans_br33
+ trans_br41 trans_br42 trans_br43 trans_br44
  trans_step
  trans_brS21 trans_brS22
  trans_brS31 trans_brS32 trans_brS33
@@ -1736,7 +1764,7 @@ Create HintDb trans.
 
 #[global] Hint Constructors is_val : trans.
 #[global] Hint Resolve
-  is_val_tau is_val_obs
+  is_val_τ is_val_obs
   wf_val_val wf_val_nonval wf_val_trans : trans.
 
 Ltac etrans := eauto with trans.
